\subsection{1D Rad Inf derivation}

We follow Carslaw and Jaeger Chapter 14.2 II.


\paragraph{Diffusion equation}
\begin{align}
  \pd{v}{t} = D_1 \pdd{v}{z}.
\end{align}


\paragraph{Boundary conditions}
\begin{align}
  \left.D_1\pd{v}{z}\right |_{z=0} &= k_+ v|_{z=0}
  \qquad (h = k_+/D_1),\\
  v |_{z\to\infty}&=0.
\end{align} 


\paragraph{Initial condition}
\begin{align}
  v(z,t'|z',t') = \delta(z-z') \qquad (0 \leq z').
\end{align}


\paragraph{Seperation of free particle solution}
The solution to this equation we will write as the sum of two parts
\begin{align}
  v=u+w.
\end{align}
Here $u$ is the sollution as if there were no boundary at $z=0$; the free 
particle solution
\begin{align}
  u(x,t|z',t'=0) = \frac{1}{2\sqrt{\pi D_1t}} e^{-(z-z')^2/(4 D_1 t)}.
\end{align}

And $w$, the correction term, is the part of $v$ that should make it conform 
with the boundary condition at $z=0$. Also, $w$ itself should go to $0$ at 
$t=t'$, so that it doesn't interfere with $u$ which already accounts for the 
initial condition.  

This time we use the Laplace Transform method, because the method of images 
only works for absorbing boundary conditions. To find $w$, we first transform 
our time-coordinate $t$ to Laplace coordinate $s$.


\paragraph{Laplace transform}
Transforming a problem into Laplace space, $F(s) = \mathcal{L}\{f(t)\}$, makes 
it easier to solve. $u(z,t)$ then becomes
\begin{align}
  \bar{u}(z,q) = \frac{1}{2D_1q} e^{-q|z-z'|}
  \qquad (q=\sqrt{s/D_1}).
\end{align}
And $\bar{w}$ now has to satisfy the differential equation
\begin{align}
  \frac{d^2\bar{w}}{dz^2} - q^{2}\bar{w} = 0.
\end{align}
Of the 2 generic solutions $e^{qz}$ goes to infinity for $z$ to infinity, so 
we are left with $Ae^{-qz}$. Combining this with $\bar{u}$ gives
\begin{align}
  \bar{v}(z) &= \bar{u}(z) + \bar{w}(z)\\
  &= \frac{1}{2D_1q} e^{-q|z-z'|} + A e^{-qz}.
\end{align}
We need to pick $A$ such that the complete solution $v$ in Laplace coordinates
satisfies the also transformed boundary condition at $z=0$, that is
\begin{align}
  \left.\pd{\bar{v}}{z}\right|_{z=z'} = h\bar{v}|_{z=z'}
\end{align}
Solving for $A$ gives
\begin{align}
  A &= \frac{1}{(q+h)}\frac{(q-h)}{2D_1q}e^{-qz'}\\
  &=\{ \frac{1}{2D_1q} - \frac{h}{D_1 q(q+h)} \}e^{-q(z')},
\end{align}
and so the solution $\bar{v}$ becomes
\begin{align}
  \bar{v} = \frac{1}{2D_1q} e^{-q|z-z'|}
  + \frac{1}{2D_1q} e^{-q(z+z')} - \frac{h}{D_1 q (q+h)}e^{-q(z+z')}.
\end{align}


\paragraph{Inverse Laplace transform}
Looking up the inverse Laplace transform, $f(t) = \mathcal{L}^{-1}\{F(s)\}$,  
of these 3 terms in a Laplace transforms table gives us the solution as given 
in the next section.
